code/poly1305/Hacl.Poly1305_512.fst
@@ -1,0 +1,23 @@
+module Hacl.Poly1305_512
+
+open FStar.HyperStack
+open FStar.HyperStack.All
+
+open Lib.IntTypes
+open Lib.Buffer
+
+open Hacl.Impl.Poly1305.Fields
+open Hacl.Impl.Poly1305
+open Hacl.Meta.Poly1305
+
+friend Hacl.Meta.Poly1305
+
+let poly1305_init = poly1305_init #M512
+
+let poly1305_update1 = poly1305_update1 #M512
+
+let poly1305_update = poly1305_update #M512
+
+let poly1305_finish = poly1305_finish #M512
+
+let poly1305_mac = poly1305_poly1305_mac_higher #M512 True poly1305_finish poly1305_update poly1305_init
